Updated cps.v and eval.v to correspond to the new syntax and semantics. Fixed most of the L6 related files including the closure conversion and hoisting transformations and proofs.

theories/L6_PCPS/closure_conversion_corresp.v
@@ -14,11 +14,7 @@ Open Scope fun_scope.
 (** * Correspondance of the relational and the computational definitions of  closure conversion *)
 
 Section CC_correct.
-  Context (utag : tag) (* Tag for types with unique constructor *)
-          (env_tag : tag) (* Tag for the type of environments *)
-          (tag_bij : tag -> tag) (* mapping from function tags to closure 
-                                    records tags *)
-          (unknown_type : type).
+  Variable (clo_tag : cTag).
 
 
   Open Scope ctx_scope.
@@ -29,16 +25,16 @@ Section CC_correct.
 
   (** Free variable map invariant *)
   Definition FVmap_inv (FVmap : VarInfoMap) Scope Funs FVs : Prop :=
-    Same_set _ Scope (fun x => exists t, M.get x FVmap = Some (BoundVar t)) /\
+    Same_set _ Scope (fun x => M.get x FVmap = Some BoundVar) /\
     Same_set _ (Setminus _ Funs Scope)
-             (fun x => exists x' t t', M.get x FVmap = Some (MRFun x' t t')) /\
+             (fun x => exists x', M.get x FVmap = Some (MRFun x')) /\
     forall N x, (nthN FVs N = Some x /\ ~ In _ Scope x /\ ~ In _ Funs x) <->
-           (exists t, M.get x FVmap = Some (FVar N t)).
+           (M.get x FVmap = Some (FVar N)).
 
   (** Function names substitution *)
   Definition subst (FVmap : VarInfoMap) x : var :=
     match M.get x FVmap with
-      | Some (MRFun x' _ _) => x'
+      | Some (MRFun x') => x'
       | _ => x
     end.
 
@@ -52,16 +48,16 @@ Section CC_correct.
 
   (** Spec for [get_name] *)
   Lemma get_name_fresh S :
-    {{ fun s => fresh S (fst s) }}
+    {{ fun s => fresh S (next_var s) }}
       get_name
-    {{ fun _ x s' => fresh S x /\ fresh (Setminus var S (Singleton var x)) (fst s') }}.  
+    {{ fun _ x s' => fresh S x /\ fresh (Setminus var S (Singleton var x)) (next_var s') }}.  
   Proof.   
     eapply pre_post_mp_l.
     eapply bind_triple. eapply get_triple.
-    intros [x d] [x' d'].
+    intros[x c i e] [x' c' i' e'].
     eapply pre_post_mp_l. eapply bind_triple.
-    eapply put_triple. intros u [x'' d'']. eapply return_triple.
-    intros [x''' d'''] Heq1 [Heq2 Heq3] H. inv Heq1. inv Heq2. inv Heq3. 
+    eapply put_triple. intros u [x'' c'' i'' e'']. eapply return_triple. 
+    intros [x''' c''' i''' e'''] Heq1 [Heq2 Heq3] H; subst. inv Heq1. inv Heq2. inv Heq3. 
     split; eauto. intros y Hleq.
     constructor.
     - eapply H. simpl in *. zify. omega.
@@ -77,132 +73,123 @@ Section CC_correct.
     intros Hinc Hf x' Hleq. eapply Hinc. eapply Hf. eassumption.
   Qed.  
   
-  Lemma FVmap_inv_set_bound FVmap Scope Funs FVs x t :
+  Lemma FVmap_inv_set_bound FVmap Scope Funs FVs x :
     FVmap_inv FVmap Scope Funs FVs ->
-    FVmap_inv (M.set x (BoundVar t) FVmap) (Union _ (Singleton _ x) Scope) Funs FVs.
+    FVmap_inv (M.set x BoundVar FVmap) (Union _ (Singleton _ x) Scope) Funs FVs.
   Proof. 
     intros [H1 [H2 H3]]. repeat split.
     - intros y Hin. destruct (Coqlib.peq y x); subst.
-      + eexists. now rewrite M.gsspec, Coqlib.peq_true.
+      + unfold In. now rewrite M.gss.
       + inv Hin. inv H; congruence.
         eapply H1 in H. edestruct H as [t' Heq].
-        eexists.  rewrite M.gsspec, Coqlib.peq_false; eauto.
+        unfold In. rewrite M.gso; now eauto.
     - intros y Hin. destruct (Coqlib.peq y x); subst.
       + eauto.
-      + edestruct Hin as [t' Heq]. rewrite M.gsspec, Coqlib.peq_false in Heq; [| now eauto ].
-        right. eapply H1. eexists; eauto.
+      + unfold In in Hin. rewrite M.gso in Hin; [| now eauto ].
+        right. eapply H1. eauto.
     - intros y Hin. inv Hin. destruct (Coqlib.peq y x); subst.
       + exfalso. eauto.
       + edestruct H2 as [H2' _].
-        edestruct H2' as [x' [t' [t'' Heq]]].
+        edestruct H2' as [x' Heq].
         * constructor; eauto.
-        * eexists.  rewrite M.gsspec, Coqlib.peq_false; eauto.
-    - eapply H2. destruct H as [x' [t' [t'' Heq]]].
+        * eexists. rewrite M.gso; eauto.
+    - eapply H2. destruct H as [x' Heq].
       destruct (Coqlib.peq x x0); subst.
-      + rewrite M.gsspec, Coqlib.peq_true in Heq. congruence.
-      + repeat eexists. rewrite M.gsspec, Coqlib.peq_false in Heq; eauto.
-    - intros Hc. destruct H as [x' [t' [t'' Heq]]].
+      + rewrite M.gss in Heq. congruence.
+      + repeat eexists. rewrite M.gso in Heq; eauto.
+    - intros Hc. destruct H as [x' Heq].
       destruct (Coqlib.peq x0 x); subst.
-      + rewrite M.gsspec, Coqlib.peq_true in Heq. congruence.
+      + rewrite M.gss in Heq. congruence.
       + inv Hc. inv H; congruence.
         eapply H2; eauto. repeat eexists.
-        rewrite M.gsspec, Coqlib.peq_false in Heq; eauto.
+        rewrite M.gso in Heq; eauto.
     - intros [Hnth [Hnin Hnin']].
       destruct (Coqlib.peq x0 x); subst.
       + exfalso. eauto. 
-      + edestruct H3 as [[t' Heq] _].
-        now repeat split; eauto.
-        eexists. rewrite M.gsspec, Coqlib.peq_false; eauto.
-    - edestruct H as [t' Heq]. 
-      destruct (Coqlib.peq x0 x); subst.
-      + rewrite M.gsspec, Coqlib.peq_true in Heq. congruence.
+      + edestruct H3 as [Heq _].
+        rewrite M.gso; eauto. eapply Heq; repeat split; eauto.
+    - destruct (Coqlib.peq x0 x); subst.
+      + rewrite M.gss in H. congruence.
       + eapply H3; eauto.
-        rewrite M.gsspec, Coqlib.peq_false in Heq; eauto.
-    - edestruct H as [t' Heq]. 
-      destruct (Coqlib.peq x0 x); subst.
-      + rewrite M.gsspec, Coqlib.peq_true in Heq. congruence.
+        rewrite M.gso in H; eauto.
+    - destruct (Coqlib.peq x0 x); subst.
+      + rewrite M.gss in H. congruence.
       + intros Hc. inv Hc. inv H0; congruence.
-        rewrite M.gsspec, Coqlib.peq_false in Heq; eauto.
+        rewrite M.gso in H; eauto.
         edestruct H3 as [_ [_ [Hc _]]].
         eapply H3 in H0; eauto. contradiction.
-    - edestruct H as [t' Heq]. 
-      destruct (Coqlib.peq x0 x); subst.
-      + rewrite M.gsspec, Coqlib.peq_true in Heq. congruence.
+    - destruct (Coqlib.peq x0 x); subst.
+      + rewrite M.gss in H. congruence.
       + intros Hc.
-        rewrite M.gsspec, Coqlib.peq_false in Heq; eauto.
+        rewrite M.gso in H; eauto.
         edestruct H3 as [_ [_ [_ Hc']]].
         eapply H3 in Hc; eauto. contradiction.
   Qed.
 
-  Lemma FVmap_inv_set_funs FVmap Scope Funs FVs x x' t t' :
+  Lemma FVmap_inv_set_funs FVmap Scope Funs FVs x x' :
     ~ In _ Scope x ->
     FVmap_inv FVmap Scope Funs FVs ->
-    FVmap_inv (M.set x (MRFun x' t t') FVmap) Scope (Union _ (Singleton _ x) Funs) FVs.
+    FVmap_inv (M.set x (MRFun x') FVmap) Scope (Union _ (Singleton _ x) Funs) FVs.
   Proof. 
     intros Hnin [H1 [H2 H3]]. repeat split.
     - intros y Hin. destruct (Coqlib.peq y x); subst.
       + contradiction.
       + eapply H1 in Hin. edestruct Hin as [t'' Heq].
-        eexists.  rewrite M.gsspec, Coqlib.peq_false; eauto.
+        unfold In. rewrite M.gso; eauto.
     - intros y Hin. destruct (Coqlib.peq y x); subst.
-      + edestruct Hin as [t'' Heq]. rewrite M.gss in Heq; congruence.
-      + edestruct Hin as [t'' Heq]. rewrite M.gso in Heq; [| now eauto ].
-        eapply H1. eexists; eauto.
+      + unfold In in Hin. rewrite M.gss in Hin; congruence.
+      + unfold In in Hin. rewrite M.gso in Hin; [| now eauto ].
+        now eapply H1.
     - intros y Hin. inv Hin. destruct (Coqlib.peq y x); subst.
       + repeat eexists. rewrite M.gss. reflexivity.
       + edestruct H2 as [H2' _].
-        edestruct H2' as [x'' [t'' [t''' Heq]]].
+        edestruct H2' as [x'' Heq].
         inv H. inv H4; congruence. constructor; eassumption.
         repeat eexists. rewrite M.gso; eassumption.
     - destruct (Coqlib.peq x0 x); subst; eauto. right.
-      eapply H2. edestruct H as [x'' [t1 [t2 Hget]]].
+      eapply H2. edestruct H as [x'' Hget].
       rewrite M.gso in Hget; [| now eauto ].
       repeat eexists; eauto. 
-    - destruct H as [x'' [t1 [t2 Hget]]].
+    - destruct H as [x'' Hget].
       destruct (Coqlib.peq x0 x); subst; eauto.
       rewrite M.gso in Hget; [| now eauto ].
-      intros Hc. apply H1 in Hc. edestruct Hc as [t3 Hget']. congruence.
+      intros Hc. apply H1 in Hc. congruence.
     - intros [Hnth [Hnin1 Hnin2]].
       destruct (Coqlib.peq x0 x); subst.
       + exfalso. eauto.
-      + edestruct H3 as [[t1 Heq] _].
-        now repeat split; eauto.
-        eexists. rewrite M.gsspec, Coqlib.peq_false; eauto.
-    - edestruct H as [t1 Heq].
-      destruct (Coqlib.peq x0 x); subst.
-      + rewrite M.gsspec, Coqlib.peq_true in Heq. congruence.
+      + edestruct H3 as [Heq _].
+        rewrite M.gso; eauto. eapply Heq; repeat split; eauto.
+    - destruct (Coqlib.peq x0 x); subst.
+      + rewrite M.gss in H. congruence.
       + eapply H3; eauto.
-        rewrite M.gsspec, Coqlib.peq_false in Heq; eauto.
-    - edestruct H as [t1 Heq].
-      destruct (Coqlib.peq x0 x); subst.
-      + rewrite M.gss in Heq. congruence.
+        rewrite M.gso in H; eauto.
+    - destruct (Coqlib.peq x0 x); subst.
+      + rewrite M.gss in H. congruence.
       + intros Hc.
-        rewrite M.gso in Heq; eauto. eapply H1 in Hc. 
-        edestruct Hc as [t2 Heq']. congruence.
-    - edestruct H as [t1 Heq].
-      destruct (Coqlib.peq x0 x); subst.
-      + rewrite M.gss in Heq. congruence.
-      + intros Hc.
-        rewrite M.gso in Heq; eauto.
-        inv Hc. inv H0; congruence.
-        edestruct H2 as [H2' _].  edestruct (H2' x0) as [y [t2 [t3 Hge']]].
-        constructor. eauto. intros Hc. eapply H1 in Hc. 
-        edestruct Hc as [t2 Heq']. congruence.
+        rewrite M.gso in H; eauto. eapply H1 in Hc. 
         congruence.
+    - destruct (Coqlib.peq x0 x); subst.
+      + rewrite M.gss in H. congruence.
+      + intros Hc.
+        rewrite M.gso in H; eauto.
+        inv Hc. inv H0; congruence.
+        edestruct H2 as [H2' _].  edestruct (H2' x0) as [y Hge'].
+        constructor. eauto. intros Hc. eapply H1 in Hc. 
+        congruence. congruence.
   Qed.
 
   (** Spec for [get_var] *)
-  Lemma get_var_project_var_sound Scope Funs Γ FVs FVmap S x :
+  Lemma get_var_project_var_sound Scope Funs c Γ FVs FVmap S x :
     binding_in_map (Singleton _ x) FVmap ->
     (* binding_not_in_map (Union _ S (Singleton _ Γ)) FVmap -> *)
     FVmap_inv FVmap Scope Funs FVs ->
-    {{ fun s => fresh S (fst s) }}
-      get_var utag x FVmap Γ
+    {{ fun s => fresh S (next_var s) }}
+      get_var clo_tag x FVmap c Γ
     {{ fun _ t s' =>
          exists C S', 
-           fresh S' (fst s') /\
-           let '(x', _, f) := t in
-           project_var Scope Funs (subst FVmap) Γ FVs S x x' C S' /\
+           fresh S' (next_var s') /\
+           let '(x', f) := t in
+           project_var clo_tag Scope Funs (subst FVmap) c Γ FVs S x x' C S' /\
            is_exp_ctx f C }}.
   Proof.
     intros Hin Minv. destruct Minv as [Minv1 [Minv2 Minv3]]. 
@@ -211,7 +198,7 @@ Section CC_correct.
     - eapply bind_triple.
       + eapply get_name_fresh.     
       + intros x' s. eapply return_triple. intros s' [Hf Hf'].
-        eexists (Eproj_c x' t n Γ Hole_c). repeat eexists. 
+        eexists (Eproj_c x' _ n Γ Hole_c). repeat eexists. 
         * eassumption.
         * edestruct Minv3 as [H1 [H2 [H3 H4]]]. now repeat eexists; eauto.
           econstructor 3; eauto.
@@ -220,31 +207,31 @@ Section CC_correct.
       + eapply get_name_fresh.  
       + intros x' s. eapply return_triple. intros s' [Hf Hf'].
         edestruct Minv2 as [H1 H2]; eauto. 
-        exists (Econstr_c x' t0 utag [v; Γ] Hole_c). repeat eexists.
+        exists (Econstr_c x' clo_tag [v; Γ] Hole_c). repeat eexists.
         * eassumption.
         * replace v with ((subst FVmap) x)
             by (unfold subst; rewrite Hget; reflexivity). 
           econstructor; eauto.
-          intros Hc. eapply Minv1 in Hc. destruct Hc as [t' Heq]. congruence.
+          intros Hc. eapply Minv1 in Hc. congruence.
           eapply H2. repeat eexists; eauto.
           eapply Hf. zify; omega.    
     - eapply return_triple. intros [s d] Hin'.      
       exists Hole_c. repeat eexists. 
       + eassumption. 
-      + constructor. eapply Minv1. eexists; eauto.
+      + constructor. eapply Minv1. eauto.
   Qed.
   
   (** Spec for [get_vars] *)
-  Lemma get_vars_project_vars_sound Scope Funs Γ FVs FVmap S xs :
+  Lemma get_vars_project_vars_sound Scope Funs c Γ FVs FVmap S xs :
     binding_in_map (FromList xs) FVmap ->
     FVmap_inv FVmap Scope Funs FVs ->
-    {{ fun s => fresh S (fst s) }}
-      get_vars utag xs FVmap Γ
+    {{ fun s => fresh S (next_var s) }}
+      get_vars clo_tag xs FVmap c Γ
     {{ fun _ t s' =>
          exists C S', 
-           fresh S' (fst s') /\
+           fresh S' (next_var s') /\
            let '(xs', f) := t in
-           project_vars Scope Funs (subst FVmap) Γ FVs S xs xs' C S' /\
+           project_vars clo_tag Scope Funs (subst FVmap) c Γ FVs S xs xs' C S' /\
            is_exp_ctx f C }}.
   Proof.
     intros Hb Hfv. eapply pre_post_mp_l.
@@ -256,14 +243,14 @@ Section CC_correct.
       + eapply get_var_project_var_sound; eauto.
         intros x Hin. eapply Hb. 
         inv Hin. constructor. eauto.
-      + intros [[x tau] f] [x' d']. eapply pre_eq_state.
-        intros [x'' d''] [C [S' [Hf [Hproj Hctx]]]].
+      + intros [x f] [x1 c1 f1 e1]. eapply pre_eq_state.
+        intros [x2 c2 f2 e2] [C [S' [Hf [Hproj Hctx]]]].
         eapply pre_post_mp_l. eapply bind_triple.
         eapply (IHxs S'); eauto.
         intros y Hin. eapply Hb. 
         constructor 2. eassumption.
-        intros [xs' f'] [x''' d''']. eapply return_triple. 
-        intros [x'''' d''''] Hyp Heq'. inversion Heq'.
+        intros [xs' f'] [x4 c4 f4 e4]. eapply return_triple.  
+        intros s5 Hyp Heq'. inversion Heq'.
         destruct Hyp as [C' [S'' [Hf' [Hproj' Hctx']]]]; eauto.
         now rewrite <- H0; eauto.
         exists (comp_ctx_f C C'), S''.
@@ -272,53 +259,16 @@ Section CC_correct.
         intros e. rewrite <- app_ctx_f_fuse. congruence.
   Qed.
   
-  (** Spec for [get_vars_with_types] *)
-  Lemma get_vars_with_types_project_vars_sound Scope Funs Γ FVs FVmap S xs :
-    binding_in_map (FromList xs) FVmap ->
-    FVmap_inv FVmap Scope Funs FVs ->
-    {{ fun s => fresh S (fst s) }}
-      get_vars_with_types utag xs FVmap Γ
-    {{ fun _ t s' =>
-         exists C S', 
-           fresh S' (fst s') /\
-           let '(xs', _, f) := t in
-           project_vars Scope Funs (subst FVmap) Γ FVs S xs xs' C S' /\
-           is_exp_ctx f C }}.
-  Proof.
-    intros Hb Hfv. eapply pre_post_mp_l.
-    revert S Hb Hfv. induction xs; intros S Hb Hfv. 
-    - eapply return_triple. intros [x' d'] _ Hf.
-      eexists Hole_c. repeat eexists; eauto. constructor.
-    - eapply pre_post_mp_r. eapply bind_triple.
-      + eapply get_var_project_var_sound; eauto.
-        intros x Hin. eapply Hb. 
-        inv Hin. constructor. eauto.
-      + intros [[x tau] f] [x' d']. eapply pre_eq_state.
-        intros [x'' d''] [C [S' [Hf [Hproj Hctx]]]].
-        eapply pre_post_mp_l. eapply bind_triple.
-        eapply (IHxs S'); eauto.
-        intros y Hin. eapply Hb. 
-        constructor 2. eassumption.
-        intros [[xs' ts'] f'] [x''' d''']. eapply return_triple. 
-        intros [x'''' d''''] Hyp Heq. inversion Heq.
-        destruct Hyp as [C' [S'' [Hf' [Hproj' Hctx']]]]; eauto.
-        now rewrite <- H0; eauto.
-        exists (comp_ctx_f C C'), S''.
-        split; [ eassumption |].
-        split. now econstructor; eauto.
-        intros e. rewrite <- app_ctx_f_fuse. congruence.
-  Qed.
-
-  Lemma subst_BoundVar_f_eq_subdomain FVmap x t S :
-    f_eq_subdomain S ((subst FVmap) {x ~> x}) (subst (M.set x (BoundVar t) FVmap)).
+  Lemma subst_BoundVar_f_eq_subdomain FVmap x S :
+    f_eq_subdomain S ((subst FVmap) {x ~> x}) (subst (M.set x BoundVar FVmap)).
   Proof.  
     intros x'. unfold subst, extend. rewrite M.gsspec.
     destruct (Coqlib.peq x' x). now eauto.
     reflexivity. 
   Qed.
 
-  Lemma subst_BoundVar_f_eq FVmap x t :
-    f_eq ((subst FVmap) {x ~> x}) (subst (M.set x (BoundVar t) FVmap)).
+  Lemma subst_BoundVar_f_eq FVmap x :
+    f_eq ((subst FVmap) {x ~> x}) (subst (M.set x BoundVar FVmap)).
   Proof.  
     intros x'. unfold subst, extend. rewrite M.gsspec.
     destruct (Coqlib.peq x' x). now eauto.
@@ -338,29 +288,29 @@ Section CC_correct.
       apply Same_set_sym. eassumption.
       constructor. intros x'. destruct (M.get x' FVmap).
       - destruct v; eauto;
-        right; intros [t' Hc]; congruence. 
-      - right. intros [t' Hc]. congruence. }
+        right; intros; congruence. 
+      - right. intros; congruence. }
     assert (Hdec2 : Decidable (Setminus _ Funs Scope)).
     { eapply Decidable_Same_set.
       apply Same_set_sym. eassumption.
       constructor. intros x'. destruct (M.get x' FVmap).
       - destruct v; eauto;
-        right; intros [y [t' [t'' Hc]]]; congruence. 
-      - right. intros [y [t' [t'' Hc]]]; congruence. }
+        right; intros [y Hc]; congruence. 
+      - right. intros [y Hc]; congruence. }
     destruct Hdec1, Hdec2.
     destruct (Dec x). 
-    - eapply Hinv1 in H1. destruct H1 as [t Heq].
-      rewrite Hb in Heq; eauto. congruence.
+    - eapply Hinv1 in H1.
+      unfold In in H1. rewrite Hb in H1; eauto. congruence.
     - destruct (Dec0 x).
-      + eapply Hinv2 in H2. destruct H2 as [y [t [t' Heq]]].
+      + eapply Hinv2 in H2. destruct H2 as [y Heq].
         rewrite Hb in Heq; eauto. congruence.
       + inv H0; try contradiction.
         inv H3. eapply H2; constructor; eauto.
         unfold In, FromList in H0.        
         edestruct In_nthN as [N Hnth]; [ eassumption |].
-        edestruct Hinv3 as [[t H'] _].
-        repeat split; eauto. intros Hin. eapply H2; constructor; eauto.
-        rewrite Hb in H'; eauto. congruence.
+        edestruct Hinv3 as [H' _].
+        assert (H3 : ~ Funs x) by (intros Hc; eapply H2; constructor; eauto).
+        specialize (H' (conj Hnth (conj H1 H3))). rewrite Hb in H'; congruence.
   Qed.
   
   Lemma binding_not_in_map_antimon (A : Type) (S S' : Ensemble M.elt) (rho : M.t A):
@@ -385,16 +335,16 @@ Section CC_correct.
 
   (** This identity is very useful to make the computation of the IH to appear
       as a subcomputation in the goal *)
-  Lemma st_eq_Ecase {S} m1 (m2 : state S (var * type * (exp -> exp))) y :
+  Lemma st_eq_Ecase {S} m1 (m2 : state S (var * (exp -> exp))) y :
     st_eq
       (ys <- m1 ;; 
        ys' <- ret (y :: ys) ;;
        t1 <- m2 ;;
-       let '(x, _ , f) := t1 in
+       let '(x, f) := t1 in
        ret (Ecase x ys', f))
       (fe <- (ys <- m1 ;;
              t1 <- m2 ;;
-             let '(x, _, f1) := t1 in    
+             let '(x, f1) := t1 in    
              ret (Ecase x ys, f1)) ;;
        match fe with
          | (Ecase x ys, f) =>
@@ -404,33 +354,13 @@ Section CC_correct.
   Proof.
     unfold pbind, ret.
     intros s. simpl. destruct (runState m1 s).
-    destruct (runState m2 s0). destruct p as [[x tau] f].
+    destruct (runState m2 s0). destruct p as [x f].
     reflexivity.
   Qed.
 
   Opaque bind ret.
 
-  Lemma get_typeinfo_preserves_prop tau P :
-    {{ fun s => P (fst s) }} get_typeinfo tau {{ fun _ _ s => P (fst s) }}.
-  Proof.
-    eapply pre_post_mp_l. eapply bind_triple. eapply get_triple.
-    intros [x t] [x' t'].
-    destruct (TDict.get tau t); eapply return_triple;
-    intros [x'' t''] H HP; inv H; inv H0; inv H1; eauto.
-  Qed.
-
-  Lemma set_typeinfo_preserves_prop t P :
-    {{ fun s => P (fst s) }} set_typeinfo t {{ fun _ _ s => P (fst s) }}.
-  Proof.
-    eapply pre_post_mp_l. eapply bind_triple. eapply get_triple.
-    intros [x d] [x' d'].
-    destruct (TDict.hash t d).
-    eapply pre_post_mp_l. eapply bind_triple. eapply put_triple.
-    intros u [x'' d'']. eapply return_triple.
-    intros [x''' t'''] H1 [H2 H3] HP; inv H1; inv H2; inv H3; eauto.
-  Qed.
-  
-  Instance FVmap_inv_Scope_Proper :
+  Global Instance FVmap_inv_Scope_Proper :
     Proper (Logic.eq ==> Same_set var ==> Logic.eq ==> Logic.eq ==> iff) FVmap_inv.
   Proof. 
     intros M1 M2 Heq1 S1 S2 Heq2 S3 S4 Heq3 l1 l2 Heq4; subst; split; intros [H1 [H2 H3]].
@@ -444,7 +374,7 @@ Section CC_correct.
       intros H. rewrite Heq2. eapply H3. eassumption. 
   Qed.
 
-  Instance FVmap_inv_Funs_Proper :
+  Global Instance FVmap_inv_Funs_Proper :
     Proper (Logic.eq ==> Logic.eq ==> Same_set var ==> Logic.eq ==> iff) FVmap_inv.
   Proof. 
     intros M1 M2 Heq1 S1 S2 Heq2 S3 S4 Heq3 l1 l2 Heq4; subst; split; intros [H1 [H2 H3]].
@@ -458,40 +388,37 @@ Section CC_correct.
       intros H. rewrite Heq3. eapply H3. eassumption. 
   Qed.
 
-  Lemma FVmapInv_add_params FVmap xs ts Scope Funs FVs :
+  Lemma FVmapInv_add_params FVmap xs Scope Funs FVs :
     FVmap_inv FVmap Scope Funs FVs ->
-    FVmap_inv (add_params xs ts FVmap) (Union _ Scope (FromList xs)) Funs FVs. 
+    FVmap_inv (add_params xs FVmap) (Union _ Scope (FromList xs)) Funs FVs. 
   Proof. 
-    revert FVmap ts Scope. induction xs; intros FVmap ts Scope Hinv.
+    revert FVmap Scope. induction xs; intros FVmap Scope Hinv.
     - rewrite FromList_nil, Union_Empty_set_l. eauto.
     - rewrite FromList_cons.
       rewrite Union_assoc; rewrite Union_sym with (s2 := Singleton M.elt a), <- Union_assoc. 
-      destruct ts; eapply FVmap_inv_set_bound; eauto.
+      eapply FVmap_inv_set_bound; eauto.
   Qed.
 
-  Lemma binding_in_map_add_params S FVmap xs ts :
+  Lemma binding_in_map_add_params S FVmap xs :
     binding_in_map S FVmap ->
-    binding_in_map (Union _ S  (FromList xs)) (add_params xs ts FVmap).
+    binding_in_map (Union _ S  (FromList xs)) (add_params xs FVmap).
   Proof.
-    revert S FVmap ts. induction xs; intros S FVmap ts Hb.
+    revert S FVmap. induction xs; intros S FVmap Hb.
     - intros x. rewrite FromList_nil, Union_Empty_set_l. eauto.
     - intros x. rewrite FromList_cons.
       rewrite Union_sym with (s2 := FromList xs), Union_assoc.
-      simpl. destruct ts; eapply binding_in_map_set; eauto. 
+      simpl. eapply binding_in_map_set; eauto. 
   Qed.
 
-  Lemma binding_not_in_map_add_params S FVmap xs ts :
+  Lemma binding_not_in_map_add_params S FVmap xs :
     binding_not_in_map S FVmap ->
     Disjoint _ S (FromList xs) ->
-    binding_not_in_map S (add_params xs ts FVmap).
+    binding_not_in_map S (add_params xs FVmap).
   Proof.
-    revert S FVmap ts. induction xs; intros S FVmap ts Hb Hd.
+    revert S FVmap. induction xs; intros S FVmap Hb Hd.
     - eauto.
     - rewrite FromList_cons in Hd.
-      destruct ts; simpl; eapply binding_not_in_map_set_not_In_S; eauto.
-      + eapply IHxs. eassumption.
-        constructor. intros x Hc. inv Hc. eapply Hd. now constructor; eauto.
-      + intros Hc. eapply Hd. eauto.
+      eapply binding_not_in_map_set_not_In_S; eauto.
       + eapply IHxs. eassumption.
         constructor. intros x Hc. inv Hc. eapply Hd. now constructor; eauto.
       + intros Hc. eapply Hd. eauto.
@@ -501,36 +428,35 @@ Section CC_correct.
     FVmap_inv (Maps.PTree.empty VarInfo) (Empty_set M.elt) (Empty_set M.elt) [].
   Proof.
     repeat split; (try now intros Hc; inv Hc); (try now intros x Hc; inv Hc). 
-    intros x Hx. destruct Hx as [t Hget]. rewrite M.gempty in Hget. now inv Hget.
-    destruct H as [x' [t [t' Hget]]]. rewrite M.gempty in Hget. now inv Hget.
-    destruct H as [t Hget]. rewrite M.gempty in Hget. now inv Hget.
+    intros x Hx. unfold In in Hx. rewrite M.gempty in Hx. now inv Hx.
+    destruct H as [x' Hget]. rewrite M.gempty in Hget. now inv Hget.
+    rewrite M.gempty in H. now inv H.
   Qed.
     
-  Lemma FVmap_inv_set_free_var FVmap Scope Funs FVs x n t:
+  Lemma FVmap_inv_set_free_var FVmap Scope Funs FVs x n:
     FVmap_inv FVmap Scope Funs FVs ->
     N.of_nat (length FVs) = n ->
     ~ In _ Scope x -> ~ In  _ Funs x -> ~ List.In x FVs ->
-    FVmap_inv (Maps.PTree.set x (FVar n t) FVmap) Scope Funs (FVs ++ [x]). 
+    FVmap_inv (Maps.PTree.set x (FVar n) FVmap) Scope Funs (FVs ++ [x]). 
   Proof.  
     intros [H1 [H2 H3]] Hlen Hnin1 Hnin2.
     split; [| split ]. 
     - split.
       + intros x' Hin. assert (Hin' := Hin).
-        eapply H1 in Hin. edestruct Hin as [t' Heq].
+        eapply H1 in Hin.
         destruct (Coqlib.peq x' x).
         subst; contradiction.
-        eexists. rewrite M.gso; eauto.
-      + intros x' [t' Hget]. eapply H1. 
-        rewrite M.gsspec in Hget. destruct (Coqlib.peq x' x).
-        subst; congruence.
-        now eauto.
+        unfold In. rewrite M.gso; eauto.
+      + intros x' Hget. eapply H1. 
+        unfold In in Hget. rewrite M.gsspec in Hget. destruct (Coqlib.peq x' x).
+        subst; congruence. now eauto.
     - split.
       + intros x' Hin. assert (Hin' := Hin). inv Hin'. 
-        eapply H2 in Hin. edestruct Hin as [y [t1 [t2 Heq]]].
+        eapply H2 in Hin. edestruct Hin as [y Heq].
         destruct (Coqlib.peq x' x).
         subst; contradiction.
         eexists. rewrite M.gso; eauto.
-      + intros x' [y [t1 [t2 Hget]]]. eapply H2. 
+      + intros x' [y Hget]. eapply H2. 
         rewrite M.gsspec in Hget. destruct (Coqlib.peq x' x).
         subst; congruence.
         now eauto.
@@ -539,53 +465,82 @@ Section CC_correct.
         destruct (nthN_app FVs [x] N) as [Hn | [Hn Hlen']].
         * destruct (Coqlib.peq x' x); subst.
           exfalso. eapply H. eapply nthN_In. rewrite <- Hnth. now eauto.
-          edestruct H3 as [[t' Hget] _].
-          repeat split; eauto. rewrite <- Hnth. now eauto.
-          eexists. now rewrite M.gso; eauto.
+          edestruct H3 as [Hget _].
+          rewrite M.gso; eauto. eapply Hget. repeat split; eauto.
+          rewrite <- Hnth. now eauto.
         * subst. rewrite Hnth in Hn. eapply nthN_is_Some_length in Hnth.
           rewrite app_length in Hnth. simpl length in *.
           destruct (N - N.of_nat (length FVs))%N eqn:Heq; simpl in Hn; try congruence.
-          inv Hn. eexists. rewrite M.gss; eauto.
+          inv Hn. rewrite M.gss; eauto.
           repeat f_equal. zify. omega. 
-      + subst. intros [t' Hget].
+      + subst. intros Hget.
         rewrite M.gsspec in Hget. destruct (Coqlib.peq x' x).
         * subst. inv Hget. repeat split; eauto.
           rewrite nthN_app_geq. rewrite N.sub_diag. reflexivity. 
           zify; omega. 
         * edestruct H3 as [_ [H1' [H2' H3']]].
-          now eexists; eauto.
+          eassumption.
           repeat split; eauto. apply nthN_is_Some_app. eassumption.
   Qed.
+
+  Lemma make_record_cTag_preserves_prop n P :
+    {{ fun s => P (next_var s) }} make_record_cTag n {{ fun _ _ s => P (next_var s) }}.
+  Proof.
+    eapply pre_post_mp_l. eapply bind_triple. eapply get_triple.
+    intros [x1 c1 f1 e1] [x2 c2 f2 e2].
+    apply pre_post_mp_l. eapply bind_triple. now apply put_triple.
+    intros x s. eapply return_triple. intros s' [[H1 H3] H2]; subst. inv H1.
+    eassumption.
+  Qed.
   
-  Lemma make_env_spec fv FVmap_o Γ_n Γ_o Scope Funs FVs S :
+  Lemma make_env_spec fv FVmap_o c Γ_n Γ_o Scope Funs FVs S :
     binding_in_map (FromList (PS.elements fv)) FVmap_o ->
     binding_not_in_map (Union M.elt S (Singleton M.elt Γ_o)) FVmap_o ->
     FVmap_inv FVmap_o Scope Funs FVs ->
-    {{ fun s => fresh S (fst s) }}
-      make_env utag env_tag fv (Maps.PTree.empty VarInfo) FVmap_o Γ_n Γ_o 
+    {{ fun s => fresh S (next_var s) }}
+      make_env clo_tag fv (Maps.PTree.empty VarInfo) FVmap_o c Γ_n Γ_o 
     {{ fun s t  s' =>
-         let '(_, FVmap_n, f) := t in
-         exists C S' FVs' tau t,
-           fresh S' (fst s') /\
-           project_vars Scope Funs (subst FVmap_o) Γ_o FVs S (PS.elements fv) FVs' C S' /\
-           is_exp_ctx f (comp_ctx_f C (Econstr_c Γ_n tau t FVs' Hole_c)) /\
+         let '(c', FVmap_n, f) := t in
+         exists C S' FVs',
+           fresh S' (next_var s') /\
+           project_vars clo_tag Scope Funs (subst FVmap_o) c Γ_o FVs S (PS.elements fv) FVs' C S' /\
+           is_exp_ctx f (comp_ctx_f C (Econstr_c Γ_n c' FVs' Hole_c)) /\
            binding_in_map (FromList (PS.elements fv)) FVmap_n /\
            binding_not_in_map (Complement _ (FromList (PS.elements fv))) FVmap_n /\
            FVmap_inv FVmap_n (Empty_set _) (Empty_set _) (PS.elements fv)
      }}.
   Proof.
-    intros Hb1 Hb2 Minv. eapply bind_triple. 
-    - eapply get_vars_with_types_project_vars_sound; eauto.
-    - intros [[xs ts] f] s1.
+    intros Hb1 Hb2 Minv. unfold make_env.
+    destruct ((fix
+                 add_fvs (l : list Maps.PTree.elt) (n : N) (map : Maps.PTree.t VarInfo)
+                 {struct l} : Maps.PTree.t VarInfo * N :=
+                 match l with
+                   | [] => (map, n)
+                   | x :: xs => add_fvs xs (n + 1)%N (Maps.PTree.set x (FVar n) map)
+                 end)
+                (PS.elements fv) 0%N (Maps.PTree.empty VarInfo)) as [map_new n] eqn:Heq.
+    eapply bind_triple.
+    - eapply get_vars_project_vars_sound; eauto.
+    - intros [xs f] s1.
       eapply pre_existential. intros C1. eapply pre_existential. intros S'.
       eapply pre_uncurry_r. intros [Hvars Hctx].
-      eapply bind_triple. now eapply set_typeinfo_preserves_prop.
+      eapply bind_triple. now eapply make_record_cTag_preserves_prop.
       intros tau s2. eapply return_triple.
-      intros s3 Hf. do 6 eexists. eassumption. 
+      intros s3 Hf. do 3 eexists. 
       repeat (split; [ eassumption |]). split.
       + intros e. rewrite Hctx. rewrite <- app_ctx_f_fuse.
-        f_equal. reflexivity.
-      + clear. 
+        now f_equal.
+      + replace map_new with
+        (fst ((fix
+                add_fvs (l : list Maps.PTree.elt) (n : N)
+                (map : Maps.PTree.t VarInfo) {struct l} :
+                Maps.PTree.t VarInfo * N :=
+                match l with
+                  | [] => (map, n)
+                  | x :: xs => add_fvs xs (n + 1)%N (Maps.PTree.set x (FVar n) map)
+                end) (PS.elements fv) 0%N (Maps.PTree.empty VarInfo)))
+          by (rewrite Heq; eauto).
+        clear.
         assert (He : FVmap_inv (Maps.PTree.empty VarInfo)
                                (Empty_set M.elt) (Empty_set M.elt) (@nil PS.elt))
           by apply FVmap_inv_empty.
@@ -623,28 +578,28 @@ Section CC_correct.
           rewrite <- app_assoc. reflexivity.
   Qed.
 
-  Lemma subst_MRFun_f_eq (FVmap : VarInfoMap) (x x' : var) (t t': type) :
-    f_eq ((subst FVmap) {x ~> x'}) (subst (M.set x (MRFun x' t t') FVmap)).
+  Lemma subst_MRFun_f_eq (FVmap : VarInfoMap) (x x' : var) :
+    f_eq ((subst FVmap) {x ~> x'}) (subst (M.set x (MRFun x') FVmap)).
   Proof.
     unfold subst. intros y. unfold extend.
     rewrite M.gsspec. destruct (Coqlib.peq y x); eauto.
   Qed.
 
 
-  Lemma make_full_closure_spec B FVmap_n FVmap_o Γ Scope Funs FVs FVs' typ S S1 S2 S1' S2' :
+  Lemma make_full_closure_spec B FVmap_n FVmap_o Γ Scope Funs FVs FVs' S S1 S2 S1' S2' :
     binding_in_map S1 FVmap_o -> 
     binding_in_map S2 FVmap_n ->
     binding_not_in_map S1' FVmap_o -> 
     binding_not_in_map S2' FVmap_n ->
     FVmap_inv FVmap_o Scope Funs FVs ->
     FVmap_inv FVmap_n (Empty_set _) (Empty_set _) FVs' ->
-    {{ fun s => fresh S (fst s) }}
-      make_full_closure utag tag_bij unknown_type B FVmap_n FVmap_o Γ typ
+    {{ fun s => fresh S (next_var s) }}
+      make_full_closure clo_tag B FVmap_n FVmap_o Γ
     {{ fun s t s' =>
          let '(FVmap_n', FVmap_o', f) := t in
          exists C S',
-           fresh S' (fst s') /\
-           make_closures B S Γ C (subst FVmap_n') S' /\
+           fresh S' (next_var s') /\
+           make_closures clo_tag B S Γ C (subst FVmap_n') S' /\
            is_exp_ctx f C /\
            f_eq_subdomain (Setminus _ Funs (Union _ Scope (name_in_fundefs B)))
                           (subst FVmap_o) (subst FVmap_o') /\
@@ -656,55 +611,47 @@ Section CC_correct.
            FVmap_inv FVmap_n' (Empty_set _) (name_in_fundefs B) FVs'
      }}.
   Proof.
-    revert FVmap_n FVmap_o Γ Scope Funs FVs FVs' typ S S1 S2 S1' S2'.
+    revert FVmap_n FVmap_o Γ Scope Funs FVs FVs' S S1 S2 S1' S2'.
     induction B;
-      intros FVmap_n FVmap_o Γ Scope Funs FVs FVs' typ S
+      intros FVmap_n FVmap_o Γ Scope Funs FVs FVs' S
              S1 S2 S1' S2' Hb1 Hb2 Hb1' Hb2'  Minv_o Minv_n. 
     - eapply bind_triple; [ now apply get_name_fresh |].
       intros x s1. eapply pre_uncurry_l. intros Hx.
       eapply bind_triple; [ eapply IHB; eassumption |].
-      intros [[FVmap_n' FVmap_o'] f] _.
+      intros [[FVmap_n' FVmap_o'] f'] _.
       eapply pre_existential. intros C. eapply pre_existential. intros S'.
       eapply pre_uncurry_r. intros [Hclo [Hctx [Hfeq [Hbn [Hbo [Hbn' [Hbo' [Minv_o' Minv_n']]]]]]]].
-      eapply bind_triple; [ now apply get_typeinfo_preserves_prop |].
-      intros t_inf s2.
-      eapply bind_triple with
-      (post' := fun _ _ s =>  fresh S' (fst s)).
-      + destruct t_inf; try now apply return_triple. 
-        eapply bind_triple. now apply set_typeinfo_preserves_prop.
-        intros. eapply bind_triple. now apply set_typeinfo_preserves_prop.
-        intros. now apply return_triple. 
-      + intros [typ' typ''] _. apply return_triple. 
-        intros s3 Hf. do 2 eexists.
-        split. eassumption. 
-        split. econstructor. eassumption. eapply Hx. zify; omega.
-        rewrite <- subst_MRFun_f_eq. reflexivity.
-        split. intros e'. simpl. rewrite Hctx. reflexivity.
-        split. rewrite <- subst_BoundVar_f_eq.
-        apply f_eq_subdomain_extend_not_In_S_r.
-        intros Hc. inv Hc. eapply H0. right. left. now eauto.
-        eapply f_eq_subdomain_antimon; [| eassumption ].
-        apply Included_Setminus_compat. now apply Included_refl.
-        apply Included_Union_compat. now apply Included_refl.
-        now apply Included_Union_r.
-        split. eapply binding_in_map_antimon; [| eapply binding_in_map_set; eassumption ].
-        simpl. rewrite (Union_sym (Singleton _ v)), Union_assoc. now apply Included_refl.
-        split.  eapply binding_in_map_antimon; [| eapply binding_in_map_set; eassumption ].
-        simpl. rewrite (Union_sym (Singleton _ v)), Union_assoc. now apply Included_refl.
-        split. eapply binding_not_in_map_set_not_In_S.
-        eapply binding_not_in_map_antimon; [| eassumption ]. 
-        apply Included_Setminus_compat. now apply Included_refl.
-        now apply Included_Union_r.
-        intros Hc. inv Hc. eapply H0. left. now eauto.
-        split. eapply binding_not_in_map_set_not_In_S.
-        eapply binding_not_in_map_antimon; [| eassumption ].
-        apply Included_Setminus_compat. now apply Included_refl.
-        now apply Included_Union_r.
-        intros Hc. inv Hc. eapply H0. left. now eauto.
-        split. simpl. rewrite <- Union_assoc. eapply FVmap_inv_set_bound.
-        eassumption.
-        simpl. apply FVmap_inv_set_funs. now apply not_In_Empty_set.
-        eassumption. 
+      apply return_triple. 
+      intros s3 Hf. do 2 eexists.
+      split. eassumption. 
+      split. econstructor. eassumption. eapply Hx. zify; omega.
+      rewrite <- subst_MRFun_f_eq. reflexivity.
+      split. intros e'. simpl. rewrite Hctx. reflexivity.
+      split. rewrite <- subst_BoundVar_f_eq.
+      apply f_eq_subdomain_extend_not_In_S_r.
+      intros Hc. inv Hc. eapply H0. right. left. now eauto.
+      eapply f_eq_subdomain_antimon; [| eassumption ].
+      apply Included_Setminus_compat. now apply Included_refl.
+      apply Included_Union_compat. now apply Included_refl.
+      now apply Included_Union_r.
+      split. eapply binding_in_map_antimon; [| eapply binding_in_map_set; eassumption ].
+      simpl. rewrite (Union_sym (Singleton _ v)), Union_assoc. now apply Included_refl.
+      split.  eapply binding_in_map_antimon; [| eapply binding_in_map_set; eassumption ].
+      simpl. rewrite (Union_sym (Singleton _ v)), Union_assoc. now apply Included_refl.
+      split. eapply binding_not_in_map_set_not_In_S.
+      eapply binding_not_in_map_antimon; [| eassumption ]. 
+      apply Included_Setminus_compat. now apply Included_refl.
+      now apply Included_Union_r.
+      intros Hc. inv Hc. eapply H0. left. now eauto.
+      split. eapply binding_not_in_map_set_not_In_S.
+      eapply binding_not_in_map_antimon; [| eassumption ].
+      apply Included_Setminus_compat. now apply Included_refl.
+      now apply Included_Union_r.
+      intros Hc. inv Hc. eapply H0. left. now eauto.
+      split. simpl. rewrite <- Union_assoc. eapply FVmap_inv_set_bound.
+      eassumption.
+      simpl. apply FVmap_inv_set_funs. now apply not_In_Empty_set.
+      eassumption. 
     - eapply return_triple. intros s Hs. do 2 eexists.
       split. eassumption. split. now constructor.
       split. intros e. reflexivity.
@@ -719,20 +666,21 @@ Section CC_correct.
       eassumption. 
   Qed.
 
-  Instance project_var_Proper Scope Funs :
+  (* Rewrite does not exactly works for these two, but they are still useful as lemmas *)
+  Global Instance project_var_Proper Scope Funs :
     Proper
-      (f_eq_subdomain (Setminus _ Funs Scope) ==> eq ==> eq ==> eq ==> eq ==> eq ==> eq ==> eq ==> iff)
-      (project_var Scope Funs).
+      (f_eq_subdomain (Setminus _ Funs Scope) ==> eq ==> eq ==> eq ==> eq ==> eq ==> eq ==> eq ==> eq ==> iff)
+      (project_var clo_tag Scope Funs).
   Proof. 
     constructor; subst; intros Hproj; inv Hproj; try (now constructor; eauto).
     - rewrite H; now econstructor; eauto.
     - rewrite <- H; now econstructor; eauto.
   Qed.
   
-  Instance project_vars_Proper Scope Funs :
+  Global Instance project_vars_Proper Scope Funs :
     Proper
-      (f_eq_subdomain (Setminus _ Funs Scope) ==> eq ==> eq ==> eq ==> eq ==> eq ==> eq ==> eq ==> iff)
-      (project_vars Scope Funs).
+      (f_eq_subdomain (Setminus _ Funs Scope) ==> eq ==> eq ==> eq ==> eq ==> eq ==> eq ==> eq ==> eq ==> iff)
+      (project_vars clo_tag Scope Funs).
   Proof. 
       constructor; subst; intros Hproj; induction Hproj; try (now constructor; eauto).
       - econstructor. eapply project_var_Proper; eauto.
@@ -741,41 +689,41 @@ Section CC_correct.
   Qed.
 
   Lemma Closure_conversion_f_eq_subdomain_mut :
-    (forall e Scope Funs σ σ' FVs Γ e' C
-       (Hcc : Closure_conversion Scope Funs σ Γ FVs e e' C)
+    (forall e Scope Funs σ σ' c FVs Γ e' C
+       (Hcc : Closure_conversion clo_tag Scope Funs σ c Γ FVs e e' C)
        (Hfeq : f_eq_subdomain (Setminus _ Funs Scope) σ σ'),
-       Closure_conversion Scope Funs σ' Γ FVs e e' C) /\
-    (forall B Funs σ σ' FVs B'
+       Closure_conversion clo_tag Scope Funs σ' c Γ FVs e e' C) /\
+    (forall B Funs σ σ' c FVs B'
        (Hinc : Included _ (name_in_fundefs B) Funs)
-       (Hcc : Closure_conversion_fundefs Funs σ FVs B B')
+       (Hcc : Closure_conversion_fundefs clo_tag Funs σ c FVs B B')
        (Hfeq : f_eq_subdomain Funs σ σ'),
-       Closure_conversion_fundefs Funs σ' FVs B B').
+       Closure_conversion_fundefs clo_tag Funs σ' c FVs B B').
   Proof. 
     eapply exp_def_mutual_ind; intros; inv Hcc.
     - econstructor; try reflexivity. rewrite <- image_f_eq_subdomain; [| eassumption ].
       eassumption.
-      eapply project_vars_Proper; [ symmetry; eassumption | | | | | | | | ];
+      eapply project_vars_Proper; [ symmetry; eassumption | | | | | | | | | ];
       try reflexivity. eassumption.
       eapply H. eassumption. eapply f_eq_subdomain_antimon; [| eassumption ].
       apply Included_Setminus_compat. now apply Included_refl.
       now apply Included_Union_r.
     - econstructor; try reflexivity. rewrite <- image_f_eq_subdomain; [| eassumption ].
       eassumption.
-      eapply project_var_Proper; [ symmetry; eassumption | | | | | | | | ];
+      eapply project_var_Proper; [ symmetry; eassumption | | | | | | | | | ];
       try reflexivity. eassumption.
-      inv H10. constructor.
+      inv H11. constructor.
     - econstructor; try reflexivity. rewrite <- image_f_eq_subdomain; [| eassumption ].
       eassumption.
-      eapply project_var_Proper; [ symmetry; eassumption | | | | | | | | ];
+      eapply project_var_Proper; [ symmetry; eassumption | | | | | | | | | ];
       try reflexivity. eassumption.
-      inv H12. inv H4. simpl in H1; subst. destruct H2 as [C' [e' [Heq Hcc]]].
+      inv H13. inv H4. simpl in H1; subst. destruct H2 as [C' [e' [Heq Hcc]]].
       constructor. now split; eauto.
-      assert (Hcc' : Closure_conversion Scope Funs σ' Γ FVs (Ecase v l)  (Ecase x' l') C).
+      assert (Hcc' : Closure_conversion clo_tag Scope Funs σ' c0 Γ FVs (Ecase v l)  (Ecase x' l') C).
       { eapply H0. econstructor; eauto. eassumption. }
       now inv Hcc'.
     - econstructor; try reflexivity. rewrite <- image_f_eq_subdomain; [| eassumption ].
       eassumption.
-      eapply project_var_Proper; [ symmetry; eassumption | | | | | | | | ];
+      eapply project_var_Proper; [ symmetry; eassumption | | | | | | | | | ];
       try reflexivity. eassumption.
       eapply H. eassumption. eapply f_eq_subdomain_antimon; [| eassumption ].
       apply Included_Setminus_compat. now apply Included_refl.
@@ -783,7 +731,7 @@ Section CC_correct.
     - econstructor; try reflexivity. eassumption.
       rewrite <- image_f_eq_subdomain; [| eassumption ].
       eassumption.
-      eapply project_vars_Proper; [ symmetry; eassumption | | | | | | | | ];
+      eapply project_vars_Proper; [ symmetry; eassumption | | | | | | | | | ];
       try reflexivity. eassumption.
       rewrite <- image_f_eq_subdomain; [| eassumption ].
       eassumption. eassumption.
@@ -796,11 +744,11 @@ Section CC_correct.
     - econstructor; try reflexivity; try eassumption.
       rewrite <- image_f_eq_subdomain; [| eassumption ].
       eassumption.
-      eapply project_vars_Proper; [ symmetry; eassumption | | | | | | | | ];
+      eapply project_vars_Proper; [ symmetry; eassumption | | | | | | | | | ];
       try reflexivity. eassumption.
     - econstructor; try reflexivity. rewrite <- image_f_eq_subdomain; [| eassumption ].
       eassumption.
-      eapply project_vars_Proper; [ symmetry; eassumption | | | | | | | | ];
+      eapply project_vars_Proper; [ symmetry; eassumption | | | | | | | | | ];
       try reflexivity. eassumption.
       eapply H. eassumption. eapply f_eq_subdomain_antimon; [| eassumption ].
       apply Included_Setminus_compat. now apply Included_refl.
@@ -817,40 +765,33 @@ Section CC_correct.
   Qed.
 
   Corollary Closure_conversion_f_eq_subdomain :
-    forall e Scope Funs σ σ' FVs Γ e' C
-       (Hcc : Closure_conversion Scope Funs σ Γ FVs e e' C)
+    forall e Scope Funs σ σ' c FVs Γ e' C
+       (Hcc : Closure_conversion clo_tag Scope Funs σ c Γ FVs e e' C)
        (Hfeq : f_eq_subdomain (Setminus _ Funs Scope) σ σ'),
-      Closure_conversion Scope Funs σ' Γ FVs e e' C.
+      Closure_conversion clo_tag Scope Funs σ' c Γ FVs e e' C.
   Proof.
     now apply Closure_conversion_f_eq_subdomain_mut.
   Qed.
 
   Corollary Closure_conversion_fundefs_f_eq_subdomain :
-  (forall B Funs σ σ' FVs B'
+  (forall B Funs σ σ' c FVs B'
        (Hinc : Included _ (name_in_fundefs B) Funs)
-       (Hcc : Closure_conversion_fundefs Funs σ FVs B B')
+       (Hcc : Closure_conversion_fundefs clo_tag Funs σ c FVs B B')
        (Hfeq : f_eq_subdomain Funs σ σ'),
-       Closure_conversion_fundefs Funs σ' FVs B B').
+       Closure_conversion_fundefs clo_tag Funs σ' c FVs B B').
   Proof. 
     now apply Closure_conversion_f_eq_subdomain_mut.
   Qed.
+  
 
-
-  Lemma subst_add_params_f_eq_subdomain S l ts FVmap :
+  Lemma subst_add_params_f_eq_subdomain S l FVmap :
     Disjoint _ (FromList l) S ->
     f_eq_subdomain S
-     (subst (add_params l ts FVmap)) (subst FVmap).
+     (subst (add_params l FVmap)) (subst FVmap).
   Proof.
-    intros Hd.
-    revert ts; induction l; intros ts.
+    intros Hd. induction l.
     - simpl. reflexivity.
-    - simpl. destruct ts.
-      rewrite <- subst_BoundVar_f_eq_subdomain.
-      eapply f_eq_subdomain_extend_not_In_S_l.
-      intros H. eapply Hd. constructor. rewrite FromList_cons.
-      now left. eassumption.
-      eapply IHl. eapply Disjoint_Included_l; [| eassumption ].
-      rewrite FromList_cons. now apply Included_Union_r.
+    - simpl.
       rewrite <- subst_BoundVar_f_eq_subdomain.
       eapply f_eq_subdomain_extend_not_In_S_l.
       intros H. eapply Hd. constructor. rewrite FromList_cons.
@@ -860,7 +801,7 @@ Section CC_correct.
   Qed.
 
   Lemma exp_closure_conv_Closure_conv_sound :
-    (forall e Scope Funs Γ FVs FVmap S
+    (forall e Scope Funs c Γ FVs FVmap S
        (* The invariant the relates [FVmap] and [Scope], [Funs], [FV] *)
        (Minv : FVmap_inv FVmap Scope Funs FVs)
        (* [FVmap] contains all the free variables *)
@@ -874,14 +815,14 @@ Section CC_correct.
        (* The current environment argument is fresh *)
        (HD2 : ~ In _ (Union _ (bound_var e) (occurs_free e)) Γ),
        {{ fun s => True }}
-         exp_closure_conv utag env_tag tag_bij unknown_type e FVmap Γ
+         exp_closure_conv clo_tag e FVmap c Γ
        {{ fun s ef s' =>
-            fresh S (fst s) ->
+            fresh S (next_var s) ->
             exists C, is_exp_ctx (snd ef) C /\
-                 Closure_conversion Scope Funs (subst FVmap) Γ FVs e (fst ef) C /\
-                 fresh S (fst s')
+                 Closure_conversion clo_tag Scope Funs (subst FVmap) c Γ FVs e (fst ef) C /\
+                 fresh S (next_var s')
        }}) /\
-    (forall B FVmap Funs FVs S
+    (forall B FVmap Funs FVs S c
        (Minv : FVmap_inv FVmap (Empty_set _) Funs FVs)
        (Hbin1 : binding_in_map (Union _ (occurs_free_fundefs B) (name_in_fundefs B)) FVmap)
        (Hbin2 : binding_not_in_map S FVmap)
@@ -889,11 +830,11 @@ Section CC_correct.
                                   (Union _ (bound_var_fundefs B) (occurs_free_fundefs B))))
        (Hinc : Included _ (name_in_fundefs B) Funs),
        {{ fun s => True }}
-         fundefs_closure_conv utag env_tag tag_bij unknown_type B FVmap
+         fundefs_closure_conv clo_tag B FVmap c
        {{ fun s B' s' =>
-            fresh S (fst s) ->       
-            Closure_conversion_fundefs Funs (subst FVmap) FVs B B' /\
-            fresh S (fst s')
+            fresh S (next_var s) ->       
+            Closure_conversion_fundefs clo_tag Funs (subst FVmap) c FVs B B' /\
+            fresh S (next_var s')
        }}).
   Proof.
     eapply exp_def_mutual_ind; intros.
@@ -901,12 +842,12 @@ Section CC_correct.
       + eapply get_vars_project_vars_sound; [ | eassumption ].
         intros x Hx. eapply Hbin1. eauto.
       + intros [xs f] s. eapply pre_eq_state.
-        intros [x'' d''] [C [S' [Hf [Hproj Hctx]]]].
+        intros [? ? ? ? ] [C [S' [Hf [Hproj Hctx]]]].
         eapply pre_post_mp_l.
         eapply bind_triple.
         eapply H with (Scope := Union var (Singleton var v) Scope)
                       (S := S')
-                      (FVmap := Maps.PTree.set v (BoundVar t) FVmap).
+                      (FVmap := Maps.PTree.set v BoundVar FVmap).
         * eapply FVmap_inv_set_bound. eassumption. 
         * eapply binding_in_map_antimon; [| eapply binding_in_map_set; eassumption ].
           now eapply occurs_free_Econstr_Included.
@@ -947,13 +888,13 @@ Section CC_correct.
           intros Hc. inv Hc. now eauto. reflexivity.
           eapply fresh_monotonic. now eapply project_vars_free_set_Included; eauto.
           eassumption.
-    - eapply pre_post_mp_r. eapply bind_triple with (post' := fun _ l i => l = [] /\ fresh S (fst i)).
+    - eapply pre_post_mp_r. eapply bind_triple with (post' := fun _ l i => l = [] /\ fresh S (next_var i)).
       + eapply return_triple; eauto. 
       + intros pats' s2.
         eapply bind_triple.
         * eapply frame_rule. eapply get_var_project_var_sound; eauto.
           intros x Hx. eapply Hbin1. rewrite occurs_free_Ecase_nil. eassumption.
-        * intros [[x tau] f] s. eapply return_triple.
+        * intros [x f] s. eapply return_triple.
           intros s' [Heq [C [S' [Hf [Hproj Hctx]]]]]. rewrite Heq.
           eexists. split; eauto. split. econstructor; [| eassumption |].
           eapply Disjoint_free_set in Minv.
@@ -985,7 +926,7 @@ Section CC_correct.
       + intros [e' f'] s'. simpl. setoid_rewrite assoc. simpl.
         setoid_rewrite st_eq_Ecase. 
         eapply pre_post_mp_l. eapply bind_triple. 
-        eapply H0 with (FVmap := FVmap) (Γ := Γ);
+        eapply H0 with (FVmap := FVmap) (Γ := Γ) (c := c0);
           [ eassumption | | eassumption | | ].
         * eapply binding_in_map_antimon; [| eassumption ].
           rewrite occurs_free_Ecase_cons. apply Included_Union_mon_r.
@@ -1008,13 +949,13 @@ Section CC_correct.
     - eapply pre_post_mp_r. eapply bind_triple.
       + eapply get_var_project_var_sound; [ | eassumption ].
         intros x Hx. inv Hx. eapply Hbin1. eauto.
-      + intros [[x tau] f] s. eapply pre_eq_state.
-        intros [x'' d''] [C [S' [Hf [Hproj Hctx]]]].
+      + intros [x f] s. eapply pre_eq_state.
+        intros [? ? ? ?] [C [S' [Hf [Hproj Hctx]]]].
         eapply pre_post_mp_l.
         eapply bind_triple.
         eapply H with (Scope := Union var (Singleton var v) Scope)
                       (S := S')
-                      (FVmap := Maps.PTree.set v (BoundVar t) FVmap).
+                      (FVmap := Maps.PTree.set v BoundVar FVmap).
         * eapply FVmap_inv_set_bound. eassumption. 
         * eapply binding_in_map_antimon; [| eapply binding_in_map_set; eassumption ].
           now eapply occurs_free_Eproj_Included.
@@ -1065,9 +1006,8 @@ Section CC_correct.
           eapply Included_Union_compat. now apply Subset_Setminus.
           now apply Included_refl.
         * eassumption.
-      + intros [[tau FVmap'] f] _. eapply pre_existential; intros C1.
+      + intros [[c' FVmap'] f] _. eapply pre_existential; intros C1.
         eapply pre_existential; intros S2. eapply pre_existential; intros FVs'.
-        eapply pre_existential; intros tau'. eapply pre_existential; intros t.
         eapply pre_uncurry_r. intros [Hproj [Hctx1 [Hb1 [Hb1' Minv1]]]].
         eapply bind_triple; [ eapply make_full_closure_spec; eassumption |].
         intros [[FVmap_n FVmap_o] f'] s2. eapply pre_existential; intros C2.
@@ -1148,15 +1088,16 @@ Section CC_correct.
             eapply Disjoint_Included_r; [| now apply HD1 ]. do 3 apply Included_Union_mon_r.
             now apply Included_refl.
             eapply binding_not_in_map_antimon; [| eassumption ]. now apply Included_Union_l. }
-          econstructor; [ | | eassumption | | eassumption | | eassumption | eassumption |  ].
+          econstructor; [ |  | eassumption | | |  | eassumption | eassumption | ]. 
           now eapply fundefs_fv_correct.
           eapply Disjoint_Included_l. now apply Subset_Setminus. 
           eapply Disjoint_Included_r; [| eassumption ].
           now apply Included_Union_r.
           eapply Disjoint_Included_l with (s8 := S).
-          intros x Hin. eapply Hin. zify. omega. eapply Disjoint_Included_r; [| eassumption ]. 
+          intros x Hin. eapply Hin. eapply Disjoint_Included_r; [| eassumption ]. 
           eapply Included_Union_compat. now apply name_in_fundefs_bound_var_fundefs.
           now apply Included_refl.
+          eapply Hf1. zify; omega.
           rewrite Union_assoc, (Union_sym _ (Singleton var Γ')), <- Union_assoc.
           eapply Disjoint_sym. eapply Disjoint_Union; eapply Disjoint_sym.
           eapply Disjoint_Included_l.
@@ -1176,7 +1117,7 @@ Section CC_correct.
         eapply binding_in_map_antimon; [| eassumption ].
         rewrite occurs_free_Eapp. apply Included_Union_mon_r.
         now apply Included_refl.
-      + intros [[x tau] f] s1. eapply pre_existential. intros C1.
+      + intros [x f] s1. eapply pre_existential. intros C1.
         eapply pre_existential. intros S'.
         eapply pre_uncurry_r. intros [Hvar Hctx1].
         eapply bind_triple.
@@ -1192,8 +1133,7 @@ Section CC_correct.
           eapply bind_triple.
           now eapply get_name_fresh. 
           intros x'' s3. eapply pre_uncurry_l. intros Hf2. 
-          eapply bind_triple. eapply get_typeinfo_preserves_prop.
-          intros tinf s4. eapply return_triple.
+          eapply return_triple.
           intros s5 Hf5. simpl. exists (comp_ctx_f C1 C2).
           split. intros e. rewrite <- app_ctx_f_fuse. congruence.
           split; eauto.
@@ -1227,7 +1167,7 @@ Section CC_correct.
         eapply bind_triple.
         eapply H with (Scope := Union var (Singleton var v) Scope)
                       (S := S')
-                      (FVmap := Maps.PTree.set v (BoundVar t) FVmap).
+                      (FVmap := Maps.PTree.set v BoundVar FVmap).
         * eapply FVmap_inv_set_bound. eassumption. 
         * eapply binding_in_map_antimon; [| eapply binding_in_map_set; eassumption ].
           now eapply occurs_free_Eprim_Included.
@@ -1280,16 +1220,14 @@ Section CC_correct.
         simpl. rewrite <- Union_assoc. apply Included_Union_compat. now apply Included_refl. 
         apply Included_Union_compat; [| now apply Included_refl ].
         now eapply name_in_fundefs_bound_var_fundefs. }
-      eapply pre_post_mp_r. eapply bind_triple.
-      now apply get_typeinfo_preserves_prop.
-      intros tau s1. eapply bind_triple. now apply get_name_fresh.
+      eapply pre_post_mp_r. eapply bind_triple. now apply get_name_fresh.
       intros x s2. apply pre_uncurry_l. intros Hf1. 
       eapply pre_post_mp_l. eapply bind_triple.
       eapply H with (Scope := FromList l) (Funs := Funs) (FVs := FVs) (S := Setminus _ S (Singleton _ x)).
       + rewrite <- Union_Empty_set_r with (s := FromList l). eapply FVmapInv_add_params.
         eassumption.
       + eapply binding_in_map_antimon; [| eapply binding_in_map_add_params; eassumption ].
-        rewrite Union_sym. rewrite Union_sym with (s3 := occurs_free_fundefs _ ).
+        rewrite Union_sym. rewrite Union_sym with (s1 := occurs_free_fundefs _).
         eapply occurs_free_in_fun. constructor. eauto.
       + intros x'. rewrite <- (@Union_Setminus _ _ _ _), Union_Included_Same_set. 
         eapply binding_not_in_map_add_params. eassumption.
@@ -1318,17 +1256,17 @@ Section CC_correct.
         * eapply Disjoint_Included_l. now apply Subset_Setminus.
           eapply Disjoint_Included_r; [| eassumption ].
           apply Included_Union_compat. now apply Included_refl.
-          rewrite bound_var_fundefs_Fcons. rewrite Union_sym with (s4 := Singleton var v).
-          do 2 rewrite <- Union_assoc. rewrite Union_sym with (s4 := Singleton var v).
+          rewrite bound_var_fundefs_Fcons. rewrite Union_sym with (s1 := Singleton var v).
+          do 2 rewrite <- Union_assoc. rewrite Union_sym with (s1 := Singleton var v).
           apply Included_Union_mon_r. (* TODO lemma *)
           apply Included_Union_compat. now apply Included_Union_r.
           now apply occurs_free_fundefs_Fcons_Included.
         * eapply Included_trans; [| eassumption ]. now apply Included_Union_r.
         * intros B' s5.
-          assert (Ha: exists v' tau1 tau2, Maps.PTree.get v FVmap = Some (MRFun v' tau1 tau2)).
+          assert (Ha: exists v', Maps.PTree.get v FVmap = Some (MRFun v')).
           { destruct Minv as [_ [HM _]]. eapply HM. rewrite Setminus_Empty_set_Same_set.
             eapply Hinc. left; eauto. }
-          destruct Ha as [v' [tau1 [tau2 Ha']]]. rewrite Ha'.
+          destruct Ha as [v' Ha']. rewrite Ha'.
           eapply return_triple. intros s6 Hcc1 Hcc2 Hf. 
           edestruct (Hcc2 Hf) as [C1 [Hctx1 [Hcc1' Hf1']]].
           destruct (Hcc1 Hf1') as [Hcc2' Hf2'].
